---
title: "EPPS Math and Coding Camp"
subtitle: "Differentiation"
author: "Instructor: Prajyna Barua and Taowen Hu"
format: 
  revealjs:
    theme: [serif]
    center: false
    slide-number: true
    logo: eppslogo.png
    css: logo.css
editor: visual
---

![](check_in.png){fig-align="center" out-width="100%"}

------------------------------------------------------------------------

## 6.2 DERIVATIVES OF FUNCTIONS

### 6.2.1 Polynomials and Powers

::: fragment
**The power rule**

$$
\frac{dx^n}{dx}=nx^{n-1}
$$
:::

------------------------------------------------------------------------

::: fragment
**The constant rule**
:::

::: fragment
$$
y=f(x)=ax
$$
:::

::: fragment
$$
f'(x)=\frac{d(ax)}{dx}=a
$$
:::

::: fragment
recall: $x^{-n}=\frac{1}{x^n}$ and $x^{\frac{1}{n}}=\sqrt[n]{x}$
:::

------------------------------------------------------------------------

::: fragment
The derivative of $e^x$ is just $e^x$:

$$
\frac{de^x}{dx}=e^x
$$
:::

------------------------------------------------------------------------

## 6.1 RULES FOR DIFFERENTIATION

### 6.1.1 The Derivative Is a Linear Operator

::: fragment
-   A linear operator satisfies pretty much the same definition. That is, an operator like $\frac{d}{dx}$ is linear if $\frac{d(f+g)}{dx}=\frac{df}{dx}+\frac{dg}{dx}$ and $\frac{d(cf)}{dx}=c\frac{df}{dx}$ for any two (differentiable!) functions $f$ and $g$ and any constant $c$.
:::

::: fragment
$$\frac{d(f+g)}{dx}=\frac{df}{dx}+\frac{dg}{dx}$$
:::

::: fragment
$$\frac{d(cf)}{dx}=c\frac{df}{dx}$$
:::

------------------------------------------------------------------------

::: fragment
-   $(f+g)'=f'+g'$ and $(f-g)'=f'-g'$
:::

::: fragment
-   $(af+bg)'=af'+bg'$ for any two constants $a$ and $b$ and any two (differentiable) functions $f$ and $g$.
:::

::: fragment
-   $h'(x)=f'(x)+g'(x)$
:::

------------------------------------------------------------------------

::: fragment
Example:

$$h(x)=x^3+6x^2+1$$
:::

::: fragment
Let's work out this last one to see the application of the rule a bit more carefully.
:::

::: fragment
$$\frac{dh(x)}{dx}=\frac{d(x^3+6x^2+1)}{dx}$$
:::

::: fragment
$$=\frac{d(x^3)}{dx}+\frac{d(6x^2)}{dx}+\frac{d(-3x)}{dx}+\frac{d(1)}{dx}$$
:::

::: fragment
$$=\frac{d(x^3)}{dx}+6 \frac{d(x^2)}{dx}-3 \frac{d(x)}{dx}+\frac{d(1)}{dx}$$
:::

::: fragment
$$=3x^2+6(2x)-3(1)+0$$
:::

::: fragment
$$=3x^2+12x-3$$
:::

------------------------------------------------------------------------

### 6.1.2 Chain Rule

::: fragment
For **composite functions** looks like $g(f(x)$, we let $f$ and $g$ be differentiable.

$$
g'(u)=g'(f(x))
$$
:::

::: fragment
$$
\frac{dg(f(x))}{dx}=\frac{dg(u)}{du} \frac{du}{dx}, \text{ where } u=f(x)
$$
:::

::: fragment
In words, take the derivative of the outer function ($g$ of $x$) evaluated at the inner function ($f$ of $x$), then take the derivative of the inner function ($f$ of $x$), and multiply the two terms.
:::

::: fragment
We can also write it as$(g(f(x)))'=g'(f(x))f'(x)$
:::

------------------------------------------------------------------------

::: fragment
Example: $h(x)=e^{2x^2}$
:::

::: fragment
We let $f(x)=2x^2$ and $g(x)=e^x$, so $h(x)=g(f(x))$
:::

::: fragment
We show below that $\frac{de^x}{dx}=e^x$ and we can use the fact that the derivative is a linear operator to find that the derivative of $2x^2$ is $2\frac{dx^2}{dx}=2(2x)=4x$
:::

::: fragment
Given this, we can apply the chain rule to get $h'(x)=g'(u)f'(x)=e^u(4x)=4xe^{2x^2}$
:::

------------------------------------------------------------------------

::: fragment
Example 2:

Let $h(x)=(2x-a)^2$
:::

::: fragment
We'll set $g(x)=x^2$ and $f(x)=(2x-a)$, so that $h(x)=g(f(x))$
:::

::: fragment
Then $h'(x)=(g(f(x)))'=g'(f(x))f'(x)=2(2x-a)(2)=8x-4a$
:::

------------------------------------------------------------------------

::: fragment
-   To get the more general case of $a^x$, we can use the properties of the exponential and logarithm to write it as $a^x=e^{x \ln (a)}$
:::

::: fragment
-   Next we use the chain rule: $g=e^x$ and $f=x \ln (a)$, so $\frac{da^x}{dx}=(e^{x \ln (a)})(\ln (a))$
:::

::: fragment
This is the **exponential rule**.
:::

------------------------------------------------------------------------

### 6.2.3 Logarithms

::: fragment
$$
\frac{d \ln (x)}{dx}=\frac{1}{x}
$$
:::

::: fragment
-   What about the more general logarithm $\log_a x$?
:::

::: fragment
This is the inverse function of $a^x$, so $a^{\log_a x}=x$
:::

::: fragment
$$
\frac{d \log_a (x)}{dx}=\frac{1}{x \ln (a)}
$$
:::

------------------------------------------------------------------------

### 6.1.3 Products Rule

::: fragment
-   one cannot always multiply out before differentiating. In such cases, the product rule is needed. If we have two functions, f(x) and g(x), then the derivative of their product is:
:::

::: fragment
$$\frac{d(f(x)g(x))}{dx}=\frac{df(x)}{dx}g(x)+f(x) \frac{dg(x)}{dx}$$
:::

::: fragment
-   The **product rule** states that the derivative of the product is a sum of product terms. In each such term, one and only one of the constituent functions is differentiated.
:::

::: fragment
Let $f$ and $g$ be differentiable functions, $(fg)'=f'g+fg'$
:::

------------------------------------------------------------------------

::: fragment
Example:

$y=f(x)g(x)=(2x+3)(x^2-15)$
:::

::: fragment
$$
\frac{dy}{dx}=\frac{d(2x+3)}{dx}(x^2-15)+(2x+3) \frac{d(x^2-15)}{dx}
$$
:::

::: fragment
$$
=(2)(x^2-15)+(2x+3)(2x)
$$
:::

::: fragment
$$
=(2x-30)+(4x^2+6x)
$$
:::

::: fragment
$$
6x^2+6x-30
$$
:::

------------------------------------------------------------------------

::: fragment
**Quotient rule** for $y=\frac{f(x)}{g(x)}$:
:::

::: fragment
$$
\frac{d}{dx} \frac{f(x)}{g(x)}=\frac{\frac{d(f(x))}{dx}g(x)-f(x) \frac{dg(x)}{dx}}{g(x)^2}
$$
:::

------------------------------------------------------------------------

::: fragment
Example:

Let $f(x)=(3x-7) \text{ and } g(x)=(x^3+6)$. We need to find $\frac{d}{dx}(\frac{3x-7}{x^3+6})$.
:::

::: fragment
$$
\frac{dy}{dx}=\frac{\frac{d(3x-7)}{dx}(x^3+6)-(3x-7) \frac{d(x^3+6)}{dx}}{(x^3+6)^2}
$$
:::

::: fragment
$$
=\frac{(x^3+6)(3)-(3x-7)(3x^2)}{36+12x^3+x^6}
$$
:::

::: fragment
$$
=\frac{(3x^3+18)-(9x^3-21x^2)}{36+12x^3+x^6}
$$
:::

::: fragment
$$
=\frac{-6x^3+21x^2+18}{36+12x^3+x^6}
$$
:::

------------------------------------------------------------------------

### 6.2.4 Other Functions

::: fragment
-   The derivatives of trigonometric functions turn them into each other, so $(\sin (x))'=\cos(x), (\cos(x))'=- \sin(x)$
:::

::: fragment
Example:

$$
f(x)= 
\begin{cases}
  -(x-2)^2 : x\leq2 \\
  \ln (x-2) : x > 2
\end{cases}
$$
:::

::: fragment
$$
f'(x)= 
\begin{cases}
  -2(x-2) : x < 2 \\
  \frac{1}{x-2} : x > 2
\end{cases}
$$ The point $x=2$ has no derivative, though it is defined for $f(x)$.
:::

------------------------------------------------------------------------

## 6.3 WHAT THE RULES ARE, AND WHEN TO USE THEM

::: fragment
**rules for differentiation**

In all these cases, $f$ and $g$ are assumed to be differentiable functions, and a is a constant.
:::

::: fragment
|                           |                                                             |
|-----------------------|------------------------------------------------|
| Sum rule                  | $(f(x)+g(x))'=f'(x)+g'(x)$                                  |
| Difference rule           | ($f(x)-g(x))'=f'(x)-g'(x)$                                  |
| Multiply by constant rule | $f'(ax)=af'(x)$                                             |
| Product rule              | $(f(x)g(x))'=f'(x)g(x)+f(x)g'(x)$                           |
| Quotient rule             | $(\frac{f(x)}{g(x)})'=\frac{f'(x)g(x)-f(x)g'(x)}{(g(x))^2}$ |
| Chain rule                | $(g(f(x))'=g'(f(x))f'(x)$                                   |
| Inverse function rule     | $(f^{-1}(x))'=\frac{1}{f'(f^{-1}x)}$                        |
| Constant rule             | $(a)'=0$                                                    |
:::

------------------------------------------------------------------------

|                     |                                    |
|---------------------|------------------------------------|
| Power rule          | $(x^n)'=nx^{n-1}$                  |
| Exponential rule 1  | $(e^x)'=e^x$                       |
| Exponential rule 2  | $(a^x)'=a^x(\ln(a))$               |
| Logarithm rule 1    | $(\ln(x))'=\frac{1}{x}$            |
| Logarithm rule 2    | $(\log_a(x))'=\frac{1}{x(\ln(a))}$ |
| Trigonometric rules | $(\sin(x))'=\cos(x)$               |
|                     | $(\cos(x))'=-\sin(x)$              |
|                     | $(\tan(x))'=1+\tan^2(x)$           |
| Piecewise rules     | Treat each piece separately        |

------------------------------------------------------------------------

## EXERCISES

### Exercise 1

::: fragment
Find the derivative of $y=f(x) \cdot g(x) = (13x+2x^3) \cdot (x^5-4x+r)$ with respect to $x$, using the rules in this chapter.
:::

::: fragment
Apply the product rule:\
$y' = f'(x) \cdot g(x) + f(x) \cdot g'(x)$
:::

::: fragment
First, compute the derivatives:

$f(x) = 13x + 2x^3 \Rightarrow f'(x) = 13 + 6x^2$\
$g(x) = x^5 - 4x + r \Rightarrow g'(x) = 5x^4 - 4$
:::

::: fragment
Now apply the rule:

$y' = (13 + 6x^2)(x^5 - 4x + r) + (13x + 2x^3)(5x^4 - 4)$
:::

------------------------------------------------------------------------

### Exercise 2

::: fragment
Differentiate the following: $$y=(x^3+x+2)^2$$
:::

::: fragment
Apply the chain rule:\
If $y = [u(x)]^2$, then $y' = 2u(x) \cdot u'(x)$\
Here, $u(x) = x^3 + x + 2$
:::

::: fragment
$u'(x) = 3x^2 + 1$

So:

$y' = 2(x^3 + x + 2)(3x^2 + 1)$
:::

------------------------------------------------------------------------

### Exercise 3

::: fragment
Differentiate the following: $$ y=
\left(\frac{x^2+1}{x+1}\right)^2
$$
:::

::: fragment
Apply the **chain rule**:\
Let $u(x) = \frac{x^2 + 1}{x + 1}$, then

$$
y = u^2 \Rightarrow y' = 2u \cdot u'
$$
:::

::: fragment
Now find $u'(x)$ using the **quotient rule**:\
If $u = \frac{f(x)}{g(x)}$, then

$$
u' = \frac{f'(x)g(x) - f(x)g'(x)}{[g(x)]^2}
$$
:::

------------------------------------------------------------------------

### Exercise 3 (continued)

::: fragment
Let: - $f(x) = x^2 + 1 \Rightarrow f'(x) = 2x$\
- $g(x) = x + 1 \Rightarrow g'(x) = 1$

So:

$$
u' = \frac{2x(x + 1) - (x^2 + 1)}{(x + 1)^2}
$$
:::

::: fragment
Now plug back into the chain rule:

$$
y' = 2 \cdot \left( \frac{x^2 + 1}{x + 1} \right) \cdot \left( \frac{2x(x + 1) - (x^2 + 1)}{(x + 1)^2} \right)
$$
:::

------------------------------------------------------------------------

### Exercise 4

::: fragment
Differentiate the following: $$
f(x)=(x^3+2) \ln(x^4-5x+3)
$$
:::

::: fragment
Apply the **product rule**:\
If $f(x) = u(x) \cdot v(x)$, then\
$$
f'(x) = u'(x)v(x) + u(x)v'(x)
$$
:::

::: fragment
Let:\
- $u(x) = x^3 + 2 \Rightarrow u'(x) = 3x^2$\
- $v(x) = \ln(x^4 - 5x + 3) \Rightarrow v'(x) = \frac{4x^3 - 5}{x^4 - 5x + 3}$
:::

::: fragment
Now apply the product rule:\
$$
f'(x) = 3x^2 \cdot \ln(x^4 - 5x + 3) + (x^3 + 2) \cdot \frac{4x^3 - 5}{x^4 - 5x + 3}
$$
:::

------------------------------------------------------------------------

### Exercise 5

::: fragment
Find the derivative of the function.
:::

::: fragment
$$                                                                                          
   y=\frac{(5 \ln(x+3))e^{3x^3-10x}}{5x^2+2}                                                               
$$
:::

::: fragment
$$                                                                                  
   y'=\frac{f'g-fg'}{g^2}=\frac{(uv)'g-fg'}{g^2}=\frac{(u'v+uv')g-fg'}{g^2}                                
$$
:::

::: fragment
$$                                                                                  
   y'=(5x^2+2)^{-2} \left[ \left( \frac{5e^{3x^3-10x}}{x+3}+5\ln(x+3)(9x^2-10)e^{3x^3-10x} \right) \\      
   \times (5x^2+2)-(5 \ln(x+3))e^{3x^3-10x}(10x) \right]                                                   
$$
:::

------------------------------------------------------------------------

![](upload_answer){fig-align="center" out-width="100%"}

------------------------------------------------------------------------

**Any Questions?**

[Home](index.html)
